experiment/Experiment.Steel.Repr.ST_to_SF.Base.fst
@@ -1,9 +1,26 @@
 module Experiment.Steel.Repr.ST_to_SF.Base
 
-module T   = FStar.Tactics
+module T = FStar.Tactics
 
 open FStar.Classical.Sugar
 open FStar.Calc
+
+
+let rec seq_sel_eq_eff_aux_sound
+      (#pre #post : Fl.ty_list) (f_eq : M.veq_eq_t (L.length pre) (L.length post))
+      (sl0 : Fl.flist pre) (sl1 : Fl.flist post) (i : nat)
+  : Lemma (requires M.veq_typ_eq pre post f_eq)
+          (ensures  seq_sel_eq_eff_aux f_eq sl0 sl1 i <==>
+                   (forall (j : Fin.fin (L.length post) {Some? (f_eq j)}) . i <= j ==> sl1 j === sl0 (Some?.v (f_eq j))))
+          (decreases L.length post - i)
+  = if i < L.length post then seq_sel_eq_eff_aux_sound f_eq sl0 sl1 (i+1)
+
+let seq_sel_eq_eff_sound
+      (#pre #post : Fl.ty_list) (f_eq : M.veq_eq_t (L.length pre) (L.length post))
+      (sl0 : Fl.flist pre) (sl1 : Fl.flist post)
+  : Lemma (requires M.veq_typ_eq pre post f_eq)
+          (ensures  seq_sel_eq_eff f_eq sl0 sl1 <==> ST.seq_sel_eq f_eq sl0 sl1)
+  = seq_sel_eq_eff_aux_sound f_eq sl0 sl1 0
 
 
 #push-options "--fuel 2 --z3rlimit 30"
@@ -61,26 +78,20 @@ and repr_SF_of_ST_ens
   = ST.match_prog_tree t
     (fun a pre post t -> (sl0 : Fl.flist pre) -> (res : a) -> (sl1 : Fl.flist (post res)) ->
        squash (ST.tree_ens t sl0 res sl1 <==> tree_ens (repr_SF_of_ST t sl0) res sl1))
-    (fun (*ST.Tequiv*) pre post0 p -> fun sl0 res sl1 -> ())
+    (fun (*ST.Tequiv*) pre post0 e -> fun sl0 res sl1 -> seq_sel_eq_eff_sound e.seq_eq sl0 sl1)
     begin fun (*ST.Tframe*) a pre post frame f -> fun sl0 x sl1 ->
-      let sl0', frame0 = Fl.splitAt_ty pre      frame sl0 in
-      let sl1', frame1 = Fl.splitAt_ty (post x) frame sl1 in
+      let sl0', sl_frame = Fl.splitAt_ty pre frame sl0 in
       calc (<==>) {
         ST.tree_ens (ST.Tframe a pre post frame f) sl0 x sl1;
-      <==> { repr_SF_of_ST_ens f sl0' x sl1' }
-        frame1 == frame0 /\ tree_ens (repr_SF_of_ST f sl0') x sl1';
-      };
-      calc (<==>) {
-        tree_ens (repr_SF_of_ST (ST.Tframe a pre post frame f) sl0) x sl1;
+      == { _ by T.(norm [delta_only [`%ST.tree_ens]; iota; zeta]; trefl ()) }
+       (let sl0', sl_frame = Fl.splitAt_ty pre frame sl0 in
+        exists (sl1' : post_v post x) .
+          ST.tree_ens f sl0' x sl1' /\ sl1 == Fl.append sl1' sl_frame);
+      <==> { FStar.Classical.forall_intro (repr_SF_of_ST_ens f sl0' x) }
+        exists (sl1' : post_v post x) .
+          tree_ens (repr_SF_of_ST f sl0') x sl1' /\ sl1 == Fl.append sl1' sl_frame;
       <==> { }
-        exists (sl1'_0 : post_v post x) .
-          tree_ens (repr_SF_of_ST f sl0') x sl1'_0 /\ sl1 == Fl.append sl1'_0 frame0;
-      <==> { introduce forall (sl1'_0 : post_v post x) .
-               sl1 == Fl.append sl1'_0 frame0 <==>
-               sl1'_0 == sl1' /\ frame1 == frame0
-             with (Fl.append_splitAt_ty (post x) frame sl1'_0 frame0;
-                   Fl.splitAt_ty_append (post x) frame sl1) }
-        tree_ens (repr_SF_of_ST f sl0') x sl1' /\ frame1 == frame0;
+        tree_ens (repr_SF_of_ST (ST.Tframe a pre post frame f) sl0) x sl1;
       }
     end
     (fun (*ST.Tspec*) a pre post req ens -> fun sl0 res sl1 -> ())
