pure/Learn.List.fst
@@ -19,11 +19,11 @@ let list_extensionality (#a : Type)
       with pf i;
     index_extensionality l0 l1
 
-let rec list_eq (#a : eqtype) (l0 l1 : list a)
-  : Tot (b : bool {b <==> l0 = l1}) (decreases l0)
+let rec list_eq (#a : Type) (eq_a : U.eq_dec a) (l0 l1 : list a)
+  : Tot (b : bool {b <==> l0 == l1}) (decreases l0)
   = match l0, l1 with
   | [], [] -> true
-  | x :: xs, y :: ys -> x = y && list_eq xs ys
+  | x :: xs, y :: ys -> x `eq_a` y && xs `list_eq eq_a` ys
   | _ -> false
 
 (* [mem_findi] *)
