pure/Learn.Option.fst
@@ -1,5 +1,14 @@
 module Learn.Option
 
+module U = Learn.Util
+
+noextract
+let opt_eq (#a : Type) (eq_a : U.eq_dec a) : U.eq_dec (option a)
+  = fun x y -> match x, y with
+  | Some x, Some y -> x `eq_a` y
+  | None, None -> true
+  | _ -> false
+
 let map #a #b (f : a -> b) (x : option a) : option b
   = match x with
   | None   -> None
