pure/Learn.Tactics.Logic.fst
@@ -1,0 +1,71 @@
+module Learn.Tactics.Logic
+
+module U = Learn.Util
+
+open FStar.Tactics
+
+
+let iff_refl (p : Type) : squash (p <==> p)
+  = ()
+
+let rew_iff_right (p q0 q1 : Type)
+    (_ : squash (q0 <==> q1))
+    (_ : squash (p  <==> q1))
+  : squash (p <==> q0)
+  = ()
+
+let conj_morph_iff (p0 q0 p1 q1 : Type0)
+    (_ : squash (p0 <==> p1))
+    (_ : squash (q0 <==> q1))
+  : squash ((p0 /\ q0) <==> (p1 /\ q1))
+  = ()
+
+let forall_morph_iff (#a : Type) (p0 p1 : a -> Type0)
+      (prf : (x : a) -> squash (p0 x <==> p1 x))
+  : squash ((forall (x : a) . p0 x) <==> (forall (x : a) . p1 x))
+  = FStar.Classical.forall_intro_squash_gtot prf
+
+let exists_morph_iff (#a : Type) (p0 p1 : a -> Type0)
+      (prf : (x : a) -> squash (p0 x <==> p1 x))
+  : squash ((exists (x : a) . p0 x) <==> (exists (x : a) . p1 x))
+  = FStar.Classical.forall_intro_squash_gtot prf
+
+let impl_morph_iff (p0 q0 p1 q1 : Type0)
+    (_ : squash (p0 <==> p1))
+    (_ : squash (q0 <==> q1))
+  : squash ((p0 ==> q0) <==> (p1 ==> q1))
+  = ()
+
+let iff_morph_iff (p0 q0 p1 q1 : Type0)
+    (_ : squash (p0 <==> p1))
+    (_ : squash (q0 <==> q1))
+  : squash ((p0 <==> q0) <==> (p1 <==> q1))
+  = ()
+
+let rew_forall_unit' (p0 : U.unit' -> Type) (p1 : Type)
+    (_ : squash (p0 U.Unit' <==> p1))
+  : squash ((forall (u : U.unit') . p0 u) <==> p1)
+  = ()
+
+let rew_exists_unit' (p0 : U.unit' -> Type) (p1 : Type)
+    (_ : squash (p0 U.Unit' <==> p1))
+  : squash ((exists (u : U.unit') . p0 u) <==> p1)
+  = ()
+
+/// Used to rewrite a [prop] to an equivalent ([<==>]) one.
+/// Solves a goal of the form [p <==> ?p']
+// TODO: currently, this can backtrack: prevent backtracking / option ?
+let rec rew_iff (pre : (unit -> Tac unit) -> Tac unit) : Tac unit =
+  let r () = rew_iff pre in
+  first [
+    (fun () -> pre r);
+    (fun () -> apply (`conj_morph_iff); iseq [r; r]);
+    // [rew_forall_unit'] needs to be done before [impl_morph_iff]
+    (fun () -> apply (`rew_forall_unit'); r ());
+    (fun () -> apply (`rew_exists_unit'); r ());
+    (fun () -> apply (`impl_morph_iff); iseq [r; r]);
+    (fun () -> apply (`forall_morph_iff); let _ = intro () in r ());
+    (fun () -> apply (`exists_morph_iff); let _ = intro () in r ());
+    (fun () -> apply (`iff_morph_iff); iseq [r; r]);
+    (fun () -> apply (`iff_refl))
+  ]
